\documentclass[12pt]{article}

% Import preambles and macros for homework
\input{../../../../preambles/hw-preamble.tex}
\input{../../../../preambles/homework-macros.tex}
\input{../../../../preambles/homework-title.tex}
\input{../../../../preambles/homework-config.tex}

\renewcommand{\author}{Deepak Jassal}
\renewcommand{\authorlast}{Jassal}
\renewcommand{\coursename}{Introductory Complex Analysis}
\renewcommand{\coursecode}{MATH 301}
\renewcommand{\assignment}{Assignment 1}
\renewcommand{\instructor}{Dr. Edward Dobrowolski}
\renewcommand{\duedate}{January 23\textsuperscript{th}, 2026}


\begin{document}
\begin{titlepage}
	\centering
	\vspace*{2.0cm}	
	\pgfornament{84}\\
	{\LARGE \textsc{\coursename}\par}
	\vspace{0.5cm}
	{\large\coursecode\par}
    \vspace{0.5cm}
    {\large\instructor\par}
	\vspace{1.5cm}
	{\huge\bfseries\assignment\par}
	\vspace{1cm}  
	{\LARGE\itshape\author\par}
    \vspace{2cm}
	{\large\bfseries Due Date:\par}
	\vspace{0.5cm}
	{\Large \duedate}\\
	\pgfornament{84}
\end{titlepage}
\stepcounter{section}
\section*{Problem 1}
Express in the form $a+bi$, $a,b\in\R$
\begin{enumerate}[label=(\alph*)]
    \item $(2+i)^4$
    \begin{align*}
		(2+4i)^4&=((2+4i)^2)^2\\
		&=(4+4i+i^2)^2\\
		&=(3+4i)^2\\
		&=9+24i^16i^2\\
		&=-7+24i.
	\end{align*}
    \item $\frac{3+4i}{4+3i}$
    \begin{align*}
		\frac{3+4i}{4+3i}&=\frac{3+4i}{4+3i}\cdot\frac{4-3i}{4-3i}\\
		&=\frac{12+7i-12i^2}{4^2+3^2}\\
		&=\frac{24+7i}{25}\\
		&=\frac{24}{25}+\frac{7}{25}i.
	\end{align*}
\end{enumerate}
\stepcounter{section}
\section*{Problem 2}
Find the three roots of $z^3-4=0$.
\[
	z^3-4=0\Leftrightarrow z^3=4.
\]
\begin{align*}
	z^3&=4\cdot e^{i2\pi n},\quad n \in\Z\\
	z_n&=4^{\frac{1}{3}}\cdot e^{\frac{i2\pi n}{3}},\quad k=0,1,2\\
	&=2^{\frac{2}{3}}\cdot e^{\frac{i2\pi n}{3}}\\
	\intertext{For $n=0$}
	z_0&=2^{\frac{2}{3}}\cdot e^{0i}=2^{\frac{2}{3}}\\
	\intertext{For $n=1$}
	z_1&=2^{\frac{2}{3}}\cdot e^{\frac{i2\pi 1}{3}}=2^{\frac{2}{3}}\left(-\frac{1}{2}+i\frac{\sqrt{3}}{2}\right)\\
	\intertext{For $n=2$}
	z_2&=2^{\frac{2}{3}}\cdot e^{\frac{i2\pi 2}{3}}=2^{\frac{2}{3}}\left(-\frac{1}{2}-i\frac{\sqrt{3}}{2}\right).
\end{align*}
\stepcounter{section}
\section*{Problem 3}
Assuming that either $|z| = 1$ or $|w| = 1$ and $\overline{z}w\neq1$, prove that
\[
    \left|\frac{z-w}{1-\overline{z}w}\right|=1.
\]
Let $E=\frac{z-w}{1-\overline{z}w}$. Then we have
\begin{align*}
	|E|^2&=E\overline{E}\\
	&=\frac{z-w}{1-\overline{z}w}\cdot\frac{\overline{z}-\overline{w}}{1-z\overline{w}}\\
	&=\frac{z\overline{z}-z\overline{w}-w\overline{z}+w\overline{w}}{1-z\overline{w}-\overline{z}w+\overline{z}w\cdot z\overline{w}}\\
	&=\frac{|z|^2-z\overline{w}-\overline{z}w+|w|^2}{1+|z|^2|w|^2-z\overline{w}-\overline{z}w}.
\end{align*}
Since both the numerator and the denominator are both positive real numbers we can take there difference, and if the difference is 0 then then we have $|E|^2=1$.
\[
	|z|^2-z\overline{w}-\overline{z}w+|w|^2-(1+|z|^2|w|^2-z\overline{w}-\overline{z}w)
\]
\[
	(|z|^2+|w|^2)-(1+|z|^2|w|^2)=|z|^2+|w|^2-1-|z|^2|w|^2.
\]
Case 1: $|z|=1$
\begin{align*}
	|z|^2+|w|^2-1-|z|^2|w|^2&=1+|w|^2-1-|w|^2\\
	&=0.
\end{align*}
Case 2: $|w|=1$
\begin{align*}
	|z|^2+|w|^2-1-|z|^2|w|^2&=1+|z|^2-1-|z|^2\\
	&=0.
\end{align*}
Since the difference between the numerator and denominator is 0 in both cases we have
\[
	|E|^2=1.
\]
Since $|E|\geq 0$ we have 
\[
	|E|=\left|\frac{z-w}{1-\overline{z}w}\right|=1.
\]
\stepcounter{section}
\section*{Problem 4}
Use complex numbers to prove identity:
\[
    1+\cos(\theta)+\cos(2\theta)+\cdots+\cos(n\theta)=\frac{1}{2}+\frac{\sin\left(\left(n+\frac{1}{2}\right)\theta\right)}{2\sin\left(\frac{\theta}{2}\right)}.
\]
\begin{proof}
	Let $z=\cos\theta+i\sin\theta$, then by De Moivre's formula $z^k=\cos^k\theta+i\sin^k\theta$. We can rewrite the sum as 
	\[
		S_n=1+\cos(\theta)+\cos(2\theta)+\cdots+\cos(n\theta)=\sum_{k=0}^{n}\cos(k\theta)=\sum_{k=0}^{n}\Re(z^k)=\Re\left(\sum_{k=0}^{n}z^k\right).
	\]
	\begin{align*}
		S_n&=\sum_{k=0}^{n}\Re(z^k)=\Re\left(\sum_{k=0}^{n}z^k\right)\\
		&=\Re(1+z+z^2+\cdots+z^n)\\
		&=\Re(1+z(1+z+\cdots+z^{n-1}))\\
		&=\Re\left(1+z\left(\frac{1-z^n}{1-z}\right)\right)\\
		&=\Re\left(1+\left(\frac{z-z^{n+1}}{1-z}\right)\right)\\
		&=\Re\left(1+\left(\frac{z-z^{n+1}}{1-z}\right)\cdot\frac{1-\overline{z}}{1-\overline{z}}\right)\\
		&=\Re\left(1+\left(\frac{z-z\overline{z}-z^{n+1}+z^nz\overline{z}}{1-\overline{z}-z+z\overline{z}}\right)\right)\\
		&=\Re\left(1+\left(\frac{z-z\overline{z}-z^{n+1}+z^nz\overline{z}}{2-2\cos\theta}\right)\right)\\
		&=\left[1+\left(\frac{\cos\theta -1 -\cos[(n+1)\theta]+\cos(n\theta)}{2-2\cos\theta}\right)\right]
	\end{align*}
	\[
		\cos(n\theta)-\cos[(n+1)\theta]=-2\sin\left(\frac{n\theta+n\theta+\theta}{2}\right)\sin\left(\frac{n\theta-n\theta-\theta}{2}\right)=2\sin[(n+1)\theta]\sin\left(\frac{\theta}{2}\right)
	\]
	\[
		1-\cos\theta=2\sin^2\left(\frac{\theta}{2}\right)\Leftrightarrow -2\sin^2\left(\frac{\theta}{2}\right)=\cos\theta-1
	\]
	\begin{align*}
		S_n&=\left[1+\frac{\cos\theta-1+2\sin\left(\left(n+\frac{1}{2}\right)\theta\right)\sin\left(\frac{\theta}{2}\right)}{2(1-\cos\theta)}\right]\\
		&=1-\frac{1}{2}+\frac{\sin\left(\left(n+\frac{1}{2}\right)\theta\right)}{2\sin\left(\frac{\theta}{2}\right)}\\
		\sum_{k=0}^{n}\cos(k\theta)&=\frac{1}{2}+\frac{\sin\left(n+\frac{1}{2}\theta\right)}{2\sin\left(\frac{\theta}{2}\right)}.\qedhere
	\end{align*}
\end{proof}	
\stepcounter{section}
\section*{Problem 5}
Solve $\sin(z)=\frac{3}{4}+i/4$.\\
\[
	\sin(z)=\frac{e^{ix}-e^{-ix}}{2i}=\frac{3}{4}+i/4.
\]
Set $w=e^{ix}$. Then,
\[
	\frac{w-w^{-1}}{2i}=\frac{3}{4}+i/4.
\]
Multiply both sides by $2i$.
\[
w-\frac{1}{w}=2i\left(\frac{3}{4} + \frac{i}{4}\right) = \frac{3i}{2} - \frac{1}{2}.
\]
Let $b=\frac{3i}{2} - \frac{1}{2}$ and multiply both sides by $w$.
\[
w^2-1=bw
\]
\[
	w^2-bw-1=0.
\]
Solving for $w$
\[
	w=\frac{-b \pm \sqrt{b^2 + 4}}{2}.
\]
\[
	b^2=\left(\frac{3i}{2} - \frac{1}{2}\right)^2= \frac{1}{4} - \frac{3i}{2} + \frac{9i^2}{4}= \frac{1}{4} - \frac{3i}{2} - \frac{9}{4} = -2 - \frac{3i}{2}.
\]
\[
	b^2+4=2 - \frac{3i}{2}=\frac{4-3i}{2}.
\]
To find $\sqrt{b^2+4}$ assume that for some $x,y\in\R$ we have $(x+iy)^2=4-3i$. Then,
\[
	(x+iy)^2=x^2 - y^2 + 2ixy=4-3i.
\]
\begin{align*}
x^2 - y^2 &= 4, \\
2xy &= -3 \quad \Rightarrow \quad xy = -\frac{3}{2}.
\end{align*}
Also $|x+iy|^2 = \sqrt{4^2 + (-3)^2} = \sqrt{16+9} = \sqrt{25} = 5$, so $x^2+y^2 = 5$.
\begin{align*}
x^2 - y^2 &= 4, \\
x^2 + y^2 &= 5.
\end{align*}
\[
	2x^2 = 9 \Rightarrow x^2 = \frac{9}{2} \Rightarrow x = \pm \frac{3}{\sqrt{2}}
\]
\[
	2y^2 = 1 \Rightarrow y^2 = \frac{1}{2} \Rightarrow y = \pm \frac{1}{\sqrt{2}}.
\]
$xy=-\frac{3}{2}$ being negative implies that $x,y$ have opposite signs, this then gives
\[
	\sqrt{4-3i} = \pm\left(\frac{3}{\sqrt{2}} - \frac{i}{\sqrt{2}}\right) = \pm\frac{3-i}{\sqrt{2}}.
\]
Thus,
\[
\sqrt{b^2+4} = \sqrt{\frac{4-3i}{2}} = \frac{\sqrt{4-3i}}{\sqrt{2}} = \frac{\pm\frac{3-i}{\sqrt{2}}}{\sqrt{2}} = \pm\frac{3-i}{2}.
\]
Solving for $w$
\[
	w = \frac{-b \pm \sqrt{b^2+4}}{2} = \frac{\frac{1}{2} - \frac{3i}{2} \pm \frac{3-i}{2}}{2}.
\]
Taking $+\frac{3-i}{2}$
\[
w_1 = \frac{\frac{1}{2} - \frac{3i}{2} + \frac{3-i}{2}}{2} = \frac{\frac{4}{2} - \frac{4i}{2}}{2} = \frac{2-2i}{2}=1-i.
\]
Taking $-\frac{3-i}{2}$
\[
w_2 = \frac{\frac{1}{2} - \frac{3i}{2} - \frac{3-i}{2}}{2} = \frac{-\frac{2}{2} - \frac{2i}{2}}{2} = \frac{-1-i}{2} = -\frac{1}{2}-\frac{1}{2}i.
\]
Recall $w = e^{iz}$, so $iz = \log(w)$
\[
z = -i\log(w) = -i\left[\ln|w| + i\arg(w) + 2\pi i n\right] = -i\ln|w| + \arg(w) + 2\pi n, \quad n \in \mathbb{Z}.
\]
$w_1$
\[
|w_1| = \sqrt{1^2+(-1)^2}= \sqrt{2}, \quad \arg(w_1) = \arctan\left(\frac{1}{-1}\right) = -\frac{\pi}{4}.
\]
So
\[
	z_1 = -i\ln\left(\sqrt{2}\right) - \frac{\pi}{4} + 2\pi n
	= -i\left(\ln\sqrt{2}\right) - \frac{\pi}{4} + 2\pi n
	= -i\ln\sqrt{2} - \frac{\pi}{4} + 2\pi n.
\]
Since $\ln\sqrt{2} = \frac{1}{2}\ln 2$
\[
z_1 = 2\pi n-\frac{\pi}{4} - \frac{i}{2}\ln 2.
\]
$w_2$
\[
|w_2| = \sqrt{\left(-\frac{1}{2}\right)^2+\left(-\frac{1}{2}\right)^2} = \sqrt{\frac{1}{2}}, \quad \arg(w_2) = \arctan\left(\frac{1}{1}\right)  = \frac{\pi}{4}.
\]
So
\[
z_2 = -i\ln\frac{1}{\sqrt{2}} + \frac{\pi}{4} + 2\pi n
= -\frac{i}{2}\ln 2 + \frac{\pi}{4} + 2\pi n.
\]
Thus,
\[
z = 2\pi n-\frac{\pi}{4} - \frac{i}{2}\ln 2 \quad \text{or} \quad z = -\frac{i}{2}\ln 2 + \frac{\pi}{4} + 2\pi n, \quad n \in \mathbb{Z}.
\]
\stepcounter{section}
\section*{Problem 6}
Find all values of $\log(-i)$.
\begin{align*}
	\log(-i)&=\log|-i|-i\frac{\pi}{2}+2\pi ni,\quad n\in\Z,\\
	&=-i\frac{\pi}{2}+2\pi ni,\quad n\in\Z.
\end{align*}
\stepcounter{section}
\section*{Problem 7}
Find all values of $1^i$.\\
$1=e^{0i+2\pi ni},$ $n\in\Z$. Thus, we can rewrite $1^i$ as 
\[
	1^i=e^{i(0i+2\pi ni)}=e^{-2\pi n}
\]
where $n\in\Z$.
\stepcounter{section}
\section*{Problem 8}
Prove that $1-\cos(2z)=2\sin^2(z)$.
\begin{proof}
From the double angle formula we know that 
\[
	\cos(2z)=\cos^2z-\sin^2z,
\]
the Pythagorean identity also tells us that
\[
	\cos^2z+\sin^2z=1.
\]
Rearranging we have
\[
	\cos^2z=1-\sin^2z.
\]
Substituting this into the double angle identity 
\[
	\cos(2z)=1-\sin^2(z)-\sin^2(z).
\]
Rearranging
\[
	1-\cos(2z)=2\sin^2(z). \qedhere
\]
\end{proof}
\stepcounter{section}
\section*{Problem 9}
Use De Moivre's formula to express $\cos(7\theta)$ in terms of $\cos(\theta)$ and $sin(\theta)$.\\
Let $z=\cos(\theta)+i\sin(\theta)$. Then by De Moivre's formula:
\begin{align*}
    z^7 &= \cos(7\theta) + i\sin(7\theta) \\
    &= (\cos(\theta) + i\sin(\theta))^7.
\end{align*}
\begin{align*}
    (\cos\theta + i\sin\theta)^7 &= \sum_{k=0}^{7} \binom{7}{k} (i\sin\theta)^k (\cos\theta)^{7-k} \\
    &= \cos^7\theta + 7i\cos^6\theta\sin\theta - 21\cos^5\theta\sin^2\theta - 35i\cos^4\theta\sin^3\theta \\
    &\quad + 35\cos^3\theta\sin^4\theta + 21i\cos^2\theta\sin^5\theta - 7\cos\theta\sin^6\theta - i\sin^7\theta.
\end{align*}
$\cos(7\theta)$ consists of the real parts of the above equation, so we have
\[
	\cos(7\theta)= \cos^7\theta- 21\cos^5\theta\sin^2\theta + 35\cos^3\theta\sin^4\theta - 7\cos\theta\sin^6\theta.
\]

\end{document}