\documentclass[12pt]{article}
\usepackage{color,soul}
% Import preambles and macros for notes
\input{../../../../preambles/notes-preamble.tex}
\input{../../../../preambles/notes-macros.tex}
\input{../../../../preambles/theorem-system-section.tex}

\title{MATH 481 Lecture 6}
\author{Deepak Jassal}
\date{January 27\textsuperscript{th}, 2026}

\begin{document}
\setcounter{section}{2}
\setcounter{tcb@cnt@mydefinition}{13}
\maketitle
\thm{Convergence of Dirichlet Series}{
    Let $f:\N\to\C$ be an arithmetic function, $F(s)$ the associated Dirichlet series and $s_f(x)=\sum_{n\leq x}f(n)$ the associated summatory function. Then,
    \begin{enumerate}[label=(\roman*)]
        \item For any $s\in\C$ with $\Re(s)>0$ such that $F(s)$ converges we have
        \[
            F(s)=s\int_{1}^{\infty}\frac{s_f(x)}{x^{s+1}}\,dx.\tag{$\ast$} \label{ast}
        \]
        \item If $S_f(x)=\Oh(x^\alpha)$ for some $\alpha\geq0$, then $F(s)$ converges then for all $s$ with $\Re(s)>\alpha$ and \eqref{ast} holds for all such $s$.
    \end{enumerate}
}
\begin{remark}
    \begin{enumerate}
        \item Let $\chi$ be a Dirichlet character ($|\chi(n)|=0$ or 1, $\chi$ is periodic).\\
        For non-trivial $\chi$, we can prove that
        \[
            \sum_{n\leq x}\chi(n)=\Oh(1).
        \]
        Let $L(s,\chi)$ be the Dirichlet series associated with $\chi$.
        \[
            L(s,\chi)=\sum_{n=1}^{\infty}\frac{\chi(n)}{n^s}.
        \]
        This is absolutly convergent for $\Re(s)>1$.\\
        By theorem 2.14(ii) and using the bound $\sum_{n\leq x}\chi(n)=\Oh(1)$ we see that $L(s,\chi)$ converges when $\Re(s)>0$.
        \item Theorem 2.14(i) can be expressed in terms of Mellin transforms.\\
        Given $\phi:\R^+\to\C$. The Mellin transform of $\phi$ is given by
        \[
            \overset{\sim}{\phi}(s)=\int_{0}^{\infty}\phi(x)x^{-s}\,dx
        \]
        ($s\in\C$) provided the integral converges.\\
        Theorem 2.14(i) can then be restated as $\dfrac{F(s)}{s}$ is the Mellin transform of $\dfrac{S_f(x)}{x}$.
    \end{enumerate}
\end{remark}
\pf[Proof of Theorem 2.14]{
    Let $s\in\C$ be such that $\Re(s)>0$ and $F(s)$ converges.\\
    (i) Consdier 
    \[
        F_N(s)=\sum\frac{f(n)}{n^s}.
    \]
    By Abel's summation formula we have
    \begin{align*}
        F_N(s)&=\left(\sum_{n\leq N}f(n)\right)N^{-s}+s\int_{1}^{N}S_f(t)t^{-s-1}\,dt\\
        &=S_f(N)N^{-s}+s\int_{1}^{\infty}S_f(N)T^{-s-1}\,dt.
    \end{align*}
    As $N\to\infty$ $F_N(s)\to F(s)$, and by \textit{theorem 2.12} $\dfrac{S_f(N)}{N^s}\to0$.\\
    So as $N\to\infty$ we get
    \[
        F(s)=s\int_{1}^{\infty}S_f(t)t^{-s-1}\,dt.
    \]
    (ii) We have
    \[
        F_N(s)=\frac{S_f(N)}{N^s}+s\int_{1}^{N}S_f(t)t^{-s-1}\,dt.
    \]
    \[
        \left|\frac{S_f(N)}{N^s}\right|=\left|\frac{S_f(N)}{N^{\Re(s)}}\right|=\Oh\left(N^{\alpha-\Re(s)}\right),
    \]
    so for $\Re(s)>\alpha$, we have $\dfrac{S_f(N)}{N^s}\to 0$ as $N\to\infty$ we also have 
    \[
        \left|\frac{S_f(t)}{t^{s+1}}\right|=\Oh(t^{\alpha-\Re(s)-1}).
    \]
    It follows that
    \begin{align*}
        \left|\int_{1}^{N}\frac{S_f(t)}{t^{s+1}}\,dt\right|&\leq\int_{1}^{N}\left|\frac{S_f(t)}{t^{s+1}}\right|\,dt\\
        &=\Oh\left(\int_{1}^{N}t^{\alpha-\Re(s)-1}\,dt\right)\\
        &=\Oh\left(N^{\alpha-\Re(s)-1}-1\right).
    \end{align*}
    Hence, $\int_{1}^{\infty}\frac{S_f(t)}{t^{s-1}}\,dt$ is convergent for $\Re(s)>\alpha$. Taking $N\to\infty$ we get $F(s)$ is convergent for $\Re(s)>\alpha$ and 
    \[
        F(s)=s\int_{1}^{\infty}\frac{S_f(t)}{t^{s-1}}\,dt
    \]
    as desired.
}
\subsection*{Convolution Method}
Say we want to compute
\[
    \sum_{n\leq x}f(x)
\]
with $f:\N\to\C$, and suppose that $f=g\ast f_0$ where both $f_0,g$ are arithmetic functions.\\
We have
\begin{align*}
    \sum_{n\leq x}f(x)&=\sum_{n\leq x}g\ast f_0(n)\\
    &=\sum_{n\leq x}\sum_{d\mid n}g(d)f_0\left(\frac{d}{n}\right)\\
    &=\sum_{d\leq x}\sum_{\substack{n\leq x\\d\mid n}}g(d)f_0\left(\frac{d}{n}\right)\\
    &=\sum_{d\leq x}\sum_{m\leq \frac{x}{d}}g(d)f_0\left(m\right)\\
    &=\sum_{d\leq x}g(d)\sum_{m\leq \frac{x}{d}}f_0\left(m\right).
\end{align*}
If an asymptotic formula is known for the last sum we substitute and proceed.\\
Let us evaluate $\sum_{n\leq x}\phi(n)$.\\
We know that $\phi(n)=\mu\ast\mathrm{id}(n)$.
\thm{Asymptotic Formula for Sum of $\phi(n)$}{
    \[
        \sum_{n\leq x}\phi(n)=\frac{3}{\pi^2}x^2+\Oh\left(x\log x\right)
    \]
}
\lemp{Sum of $\frac{\mu(n)}{n^2}$}{
    \[
        \sum_{n\leq x}\frac{\mu(n)}{n^2}=\frac{1}{\zeta(2)}.
    \]
    In general
    \[
        \sum_{n\leq x}\frac{\mu(n)}{n^s}=\frac{1}{\zeta(s)},\quad \Re(s)>1.
    \]
}{
    \[
        1=\sum_{n=1}^{\infty}\frac{e(n)}{n^2}
    \]
    where 
    \[
        e(n)=
        \begin{cases}
            1&\text{if }n=1\\
            0&\text{otherwise}.    
        \end{cases}
    \]
    \begin{align*}
        1&=\sum_{n=1}^{\infty}\frac{e(n)}{n^2}\\
        &=\sum_{n=1}^{\infty}\frac{\displaystyle\sum_{d\mid n}\mu(d)}{n^2}\\
        &=\sum_{n=1}^{\infty}\frac{1}{n^2}\sum_{d\mid n}\mu(d)\\
        &=\sum_{d=1}^\infty\mu(d)\sum_{n=1}^{\infty}\frac{1}{n^2}\\
        &=\sum_{d=1}^\infty\mu(d)\sum_{m=1}^{\infty}\frac{1}{(md)^2}\\
        1&=\sum_{d=1}^\infty\frac{\mu(d)}{d^2}\zeta(2)
    \end{align*}
}
\pf[Proof of Theorem 2.15]{
    We have
    \begin{align*}
        \sum_{n\leq x}\phi(n)&=\sum_{n\leq x}\mu\ast\mathrm{id}(n)\\
        &=\sum_{n\leq x}\sum_{d\mid n}\mu(d)\frac{d}{n}\\
        &=\sum_{d\leq x}\mu(d)\left(\sum_{m\leq\frac{n}{d}}m\right)\\
        &=\sum_{d\leq x}\mu(d)\left(\frac{\floor{\frac{x}{d}}\left(\floor{\frac{x}{d}+1}\right)}{2}\right).
    \end{align*}
    \begin{align*}
        \frac{1}{2}\floor{\frac{x}{d}}\left(\floor{\frac{x}{d}+1}\right)&=\frac{1}{2}\left(\frac{x}{d}-\fract{\frac{x}{d}}\right)\left(\frac{x}{d}-\fract{\frac{x}{d}}+1\right)\\
        &=\frac{1}{2}\left(\left(\frac{x}{d}\right)^2-2\fract{\frac{x}{d}}\frac{x}{d}+\frac{x}{d}-\fract{\frac{x}{d}}+\fract{\frac{x}{d}}^2\right)\\
        &=\frac{1}{2}\left(\frac{x}{d}\right)^2+\Oh\left(\frac{x}{d}\right).
    \end{align*}
    \begin{align*}
        \sum_{n\leq x}\phi(n)&=\sum_{d\leq x}\mu(d)\left(\frac{1}{2}\left(\frac{x}{d}\right)^2+\Oh\left(\frac{x}{d}\right)\right)\\
        &=\frac{x^2}{2}\sum_{d\leq x}\frac{\mu(d)}{d^2}+\Oh\left(\sum_{d\leq x}\frac{x}{d}\right)\\
        &=\frac{x^2}{2}\sum_{d\leq x}\frac{\mu(d)}{d^2}+\Oh(x\log x)\\
        &=\frac{x^2}{2}\left(\sum_{d=1}^{\infty}\frac{\mu(d)}{d^2}-\sum_{d> x}\frac{\mu(d)}{d^2}\right)+\Oh(x\log x)\\
        &=\frac{x^2}{2\zeta(2)}-\frac{x^2}{2}\sum_{d> x}\frac{\mu(d)}{d^2}+\Oh(x\log x).
    \end{align*}
    \begin{align*}
        \left|\sum_{d>x}\frac{\mu(d)}{d^2}\right|&\leq\sum_{d\geq\floor{x}+1}\frac{\mu(d)}{d^2}\\
        &=\int_{\floor{x}}^{\infty}\frac{dt}{t^2}\\
        &=\Oh\left(\frac{1}{x}\right).
    \end{align*}
    All in all we have
    \begin{align*}
        \sum_{n\leq x}\phi(n)&=\frac{x^2}{2\zeta(2)}+\Oh\left(x\log x\right)\\
        &=\frac{3}{\pi^2}x^2+\Oh\left(x\log x\right).
    \end{align*}
}
\subsection*{Dirichlet's Hyperbola Method}
\thm{Sum of Divisor Function}{
    \[
        \sum_{n\leq x}\mathrm{d}(n)=x\log x+(2\gamma-1)x+\Oh(\sqrt{x}).
    \]
}
\end{document}